Lamcalc/Inversion.lean
@@ -4,10 +4,8 @@ open ARS
 theorem Typed.pi_inv :
     Typed Γ (.pi a b) c ->
     ∃ i j, Typed (a :: Γ) b (.srt i) ∧ c === .srt j := by
-  generalize e: Tm.pi a b = m
-  intro ty
-  induction ty using Typed.rec (motive_2 := fun _ _ => True)
-  generalizing a b
+  generalize e: Tm.pi a b = x
+  intro ty; induction ty generalizing a b
   all_goals try trivial
   case pi i _ j _ _ _ _ =>
     cases e
@@ -23,3 +21,69 @@ theorem Typed.pi_inv :
     . apply Conv.trans
       apply Conv.sym eq1
       apply eq2
+
+theorem Typed.lam_inv' :
+    Typed Γ (.lam a m) c ->
+    c === .pi a' b ->
+    Typed (a' :: Γ) b (.srt i) ->
+    Typed (a' :: Γ) m b := by
+  generalize e: Tm.lam a m = x
+  intro ty; induction ty generalizing a m
+  all_goals try trivial
+  case lam =>
+    cases e; intro eq ty
+    have wf := ty.wf; cases wf
+    have ⟨eqa, eqb⟩ := Conv.pi_inj eq; clear eq
+    apply Typed.conv
+    . apply eqb
+    . apply Typed.conv_ctx
+      apply Conv.sym eqa
+      assumption
+      assumption
+    . assumption
+  case conv ih _ =>
+    cases e; intro eq ty
+    apply ih
+    . rfl
+    . apply Conv.trans <;> assumption
+    . assumption
+
+theorem Typed.validity : Typed Γ m a -> ∃ i, Typed Γ a (.srt i) := by
+  intro ty; induction ty
+  all_goals try trivial
+  case srt i _ _ =>
+    exists i.succ.succ
+    constructor
+    assumption
+  case var wf hs _ =>
+    have ⟨i, _⟩ := wf.has_typed hs
+    exists i
+  case pi i _ j tya _ iha ihb =>
+    exists (max i j).succ
+    constructor
+    exact tya.wf
+  case lam tym iha ihm =>
+    have wf := tym.wf
+    cases wf; case cons i _ _ =>
+    have ⟨j, _⟩ := ihm
+    exists (max i j)
+    constructor <;> assumption
+  case app _ tyn ihm _ =>
+    replace ⟨i, ihm⟩ := ihm
+    replace ⟨i, j, tyb, eq⟩ := ihm.pi_inv
+    exists i
+    apply Typed.esubst <;> try first | rfl | assumption
+    asimp
+  case conv i _ _ _ _ _ =>
+    exists i
+
+theorem Typed.lam_inv :
+    Typed Γ (.lam a m) (.pi a' b) ->
+    Typed (a' :: Γ) m b := by
+  intro ty
+  have ⟨_, ty⟩ := ty.validity
+  have ⟨_, _, ty, _⟩ := ty.pi_inv
+  apply Typed.lam_inv'
+  . assumption
+  . constructor
+  . assumption
